\documentclass[11pt]{article}
\usepackage{graphics,graphicx}
\usepackage{amsmath,amssymb}
\usepackage{tabularx}
\usepackage{times}
\usepackage{amssymb}
\usepackage[left=2cm,right=2cm,top=1.cm,bottom=2cm]{geometry}
\setlength{\parskip}{1ex} %--skip lines between paragraphs
\setlength{\parindent}{0pt} %--don't indent paragraphs
\renewcommand{\baselinestretch}{1.2}
\renewcommand{\theequation}{\arabic{equation}}


%-- Commands for header
\renewcommand{\title}[1]{\textbf{#1}\\}
\renewcommand{\line}{\begin{tabularx}{\textwidth}{X>{\raggedleft}X}\hline\\\end{tabularx}\\[-0.5cm]}
\newcommand{\leftright}[2]{\begin{tabularx}{\textwidth}{X>{\raggedleft}X}#1%
& #2\\\end{tabularx}\\[-0.5cm]}

% HEADER %
\begin{document}
\title{MATH 2800-01: Mathematics Major Seminar}
\line
\leftright{Assignment \# 08 ~~~~ 10 Dec 2025}{David Haberkorn}
% END HEADER %


\section*{Problem 1}

    \textbf{Result:} Suppose that $ \lim_{x \to a} f(x) = L$, where $L>0$. Then $ \lim_{x \to a} \sqrt{f(x)} = \sqrt{L}$.
    \\
    \textbf{Proof:} Let $\epsilon > 0$. Since $\lim_{x \to a} f(x) = L$, there exists a $\delta > 0$ such that if $0 < |x-a| < \delta$, then $|f(x) - L| < \epsilon\sqrt{L}$. \\
    Now suppose $0 < |x-a| < \delta$. We have
    \begin{align*}
        |\sqrt{f(x)} - \sqrt{L}| = \frac{|f(x)-L|}{|\sqrt{f(x)} + \sqrt{L}|} \leq \frac{|f(x)-L|}{\sqrt{L}} < \frac{\delta}{\sqrt{L}} = \frac{\sqrt{L}\epsilon}{\sqrt{L}} = \epsilon
    \end{align*}
    Thus, $ \lim_{x \to a} \sqrt{f(x)} = \sqrt{L}$. \hfill $\Box$


\newpage

\section*{Problem 2}

    \textbf{Result:} The function $Q: \mathbb{R} - \{-1\}$ is defined as
    \begin{align*}
        Q(x) = 
        \begin{cases}
        \dfrac{x^2 - 3x + 2}{x^2 - 1}, & x \in \mathbb{R} \setminus \{-1,1\}, \\[10pt]
        -\dfrac{1}{2}, & x = 1.
    \end{cases}
    \end{align*}
    $Q(x)$ is continuous at $x=1$.

    \textbf{Proof:} In order to show continuity at $x=1$, we must show that 
    \begin{enumerate}
        \item $ \lim_{x \to 1} Q(x)$ exists,
        \item $ \lim_{x \to 1} Q(x) = Q(1)$,
        \item $Q(1)$ is defined.
    \end{enumerate}
    From the definition of $Q(x)$ above, we have that $Q(1) = -\frac{1}{2}$, which satisfies the third criteria above. \\
    To show the first and second criteria, we employ an $\epsilon - \delta$ proof. \\
    Let $\epsilon > 0$, and choose $\delta = \min{1, \frac{2}{3}}\epsilon$. Now suppose $ \left| x-1 \right| < 1$.
    \begin{align*}
        \left| x-1 \right| < 1 \\
        -1 < x-1 < 1 \\
        1 < x+1 < 3
    \end{align*}
    This implies that the quantity $\left| x+1 \right| = x+1$. Now suppose $0 < \left|x-1\right| < \delta$. We have
    \begin{align*}
        \left| \frac{x^2-3x+2}{x^2-1} - \frac{-1}{2}\right| = \left| \frac{x-2}{x+1} + \frac{1}{2}\right| = \left| \frac{3(x-1)}{2(x+1)} \right| = \frac{3\left|x-1\right|}{2(x+1)} \leq \frac{3\left|x-1\right|}{2} < \frac{3\delta}{2} \leq \frac{3}{2} \cdot \frac{2}{3}\epsilon = \epsilon
    \end{align*}
    Therefore, the limit exists. \\
    Evaluating $Q(1)$, we have
    \[
    \begin{gathered}
        \frac{x^2-3x+2}{x^2-1} = \frac{x-2}{x+1} \rightarrow \frac{(1)-2}{(1)+1} = -\frac{1}{2}
    \end{gathered}
    \]
    Since the limit both exists and is equal to $Q(1)$, we have satisfied all three necessary criteria. Therefore, the function $Q(x)$ is continuous at $x=1$. \hfill $\Box$


    

\newpage

\section*{Problem 3}

    \textbf{Result:} Let $A$ be a nonempty set and let $f: A \rightarrow A$ be a function. If $f \circ f = i_a$, then $f$ is bijective.
    \\
    \textbf{Proof:} Let $A$ be a nonempty set and let $f: A \rightarrow A$ be a function, and suppose that $f \circ f = i_a$. In order to show that $f$ is bijective, we must show that $f$ is both one-to-one and onto. We start with one-to-one. \\
    Suppose that there are some elements $x, y \in A$ such that $f(x) = f(y)$. We work to show that $x = y$.
    \begin{align*}
        f(x) &= f(y) \\
        f(f(x)) &= f(f(y))
    \end{align*}
    By the definition of the identity function, we have 
    \begin{align*}
        f(f(x)) &= f(f(y)) \\
        x = y
    \end{align*}
    Thus, $f$ is one-to-one. \\
    We now work to show that $f$ is also onto. Let $r$ be an arbitrary element in $A$, and let another arbitrary element $q \in A$ be such that $f(r) = q$. We know that $q$ exists because $f$ is defined by $f: A \rightarrow A$. Through algebra, we have
    \begin{align*}
        f(r) &= q \\
        f(f(r)) &= f(q) \\
        r &= f(q)
    \end{align*}
    Since we have shown that for an arbitrary element $r$ in the codomain $A$, there exists an element $q$ in the domain $A$ (specifically $q = f(r)$) such that $f(q) = r$, the function $f$ is onto. \\
    Since $f$ is both one-to-one and onto, it is, by definition, bijective. \hfill $\Box$
\newpage


\section*{Problem 4}

    \textbf{Result:} Let the composition $ g \circ f : (0, 1) \rightarrow \mathbb{R} $ of two functions $f$ and $g$ be given by $ (g \circ f)(x) = \frac{4x-1}{2 \sqrt{x-x^2}} $ where $f: (0,1) \rightarrow (-1, 1) $ is defined by $ f(x) = 2x-1 $ for $x \in (0,1) $. The function $g$ is given by $g(y) = \frac{2y-1}{2\sqrt{1-y^2}}$.
    \\
    \textbf{Proof:} Let the function $f$ and the composition $g \circ f$ be defined as above. We work to find the function $g$. \\
    From the definitions above, we have
    \begin{align*}
        f(x) &= 2x-1 \\
        y &= 2x-1 \\
        y+1 &= 2x \\
        \frac{y+1}{2} &= x \tag{1}
    \end{align*}
    Expression (1) above is the inverse of $f(x)$, or in other words, $f^{-1}(x)$. \\
    Plugging the inverse function into the composition $(g \circ f)(x)$, we will be able to 'undo' the function $f$ to be left with $g$.
    \begin{align*}
        (g \circ f)(x) &= \frac{4x-1}{2 \sqrt{x-x^2}} \\
        g(y) &= \frac{  4(\frac{y+1}{2})-1 }{  2 \sqrt{(\frac{y+1}{2})-(\frac{y+1}{2})^2}  } \\
        g(y) &= \frac{  2y+1 }{ \sqrt{1-y^2}  }
    \end{align*}
    Thus, we have our function $g(y) = \frac{  2y+1 }{ 2 \sqrt{1-y^2}}$. \hfill $\Box$

\newpage



\section*{Problem 5}

    \textbf{Result:} Let $A = \mathbb{R} - \{1\}$ and define $f : A \rightarrow A$ by $f(x) = \frac{x}{x-1}$ for all $x \in A$. When this is the case, then $f$ is bijective, and $f^{-1} = f = \frac{x}{x-1}$.
    \\
    \textbf{Proof:} Let the function $f$ be defined as above. In order to show bijectivity, we must show injectivity and surjectivity. We begin with injectivity. \\
    Suppose there are some elements $x, y \in A$ such that $f(x) = f(y)$. We work to show that $x = y$.
    \begin{align*}
        f(x) &= f(y) \\
        \frac{x}{x-1} &= \frac{y}{y-1} \\
        x(y-1) &= y(x-1) \\
        xy - x &= xy - y \\
        -x &= -y \\
        x &= y
    \end{align*}
    Thus, $f$ is injective. \\
    To show surjectivity, let $q, r$ be arbitrary elements in $A$ such that $f(q) = r$. We work to show that there exists such a $q$.
    \begin{align*}
        f(q) &= r \\
        \frac{q}{q-1} &= r \\
        q &= (q-1)r \\
        q &= qr - r \\
        0 &= qr - q - r \\
        r &= qr - q \\
        r &= q(r-1) \\
        \frac{r}{r-1} &= q \\
        q &= \frac{r}{r-1} 
    \end{align*}
    Recalling that the domain $A$ is defined by all real numbers, excluding $\{1\}$, we see that there does in fact exist such a $q$. \\
    Since $f$ is both injective and surjective, we have that it is, in fact, bijective. \\
    \\
    In order to find the inverse of $f$, we use algebra. Let $f(x) = y$ and let $x \in A$.
    \begin{align*}
        f(x) &= \frac{x}{x-1} \\
        y &= \frac{x}{x-1} \\
    \end{align*}
    Without loss of generality (from the proof of surjectivity), we have
    \begin{align*}
        x &= \frac{y}{y-1} \\
        f^{-1}(x) &= \frac{y}{y-1}
    \end{align*}
    \hfill $\Box$
\newpage


\section*{Problem 6}

    \textbf{Result:} The sequence $ \{\frac{n+2}{2n+3}\} $ is convergent to $\frac{1}{2}$.

    \textbf{Proof:} We want to show that $ \lim_{n \to \infty} \ (\frac{n+2}{2n+3}) = \frac{1}{2}$. \\
    Let $\epsilon > 0$. By algebra, we have
    \begin{align*}
        \left| \frac{n+2}{2n+3} - \frac{1}{2} \right| &< \epsilon \\
        \left| \frac{2n+4}{4n+6} - \frac{2n+3}{4n+6} \right| &< \epsilon \\
        \left| \frac{1}{4n+6} \right| &< \epsilon \\
        \frac{1}{4n+6} &< \epsilon \\
        4n + 6 &> \frac{1}{\epsilon} \\
        n &> \frac{1}{4\epsilon}-\frac{3}{2}
    \end{align*}
    We now choose $ N = \lceil \frac{1}{4\epsilon}-\frac{3}{2} \rceil \geq (\frac{1}{4\epsilon}-\frac{3}{2}) $.
    For $n > N$, we have
    \begin{align*}
        \left| \frac{n+2}{2n+3} - \frac{1}{2} \right| = \frac{1}{4n+6} < \frac{1}{4N+6} \leq \frac{1}{4 (\frac{1}{4\epsilon}-\frac{3}{2}) +6} = \frac{1}{\frac{4}{4\epsilon} - \frac{12}{2}+6} = \frac{1}{(\frac{1}{\epsilon})} = \epsilon
    \end{align*}
    Therefore, we have that the sequence $ \{\frac{n+2}{2n+3}\} $ is convergent to $\frac{1}{2}$. \hfill $\Box$

\newpage


\section*{Problem 7}

    \textbf{Result:} $ \lim_{x \to 3} (\frac{3x+1}{4x+3}) = \frac{2}{3} $.

    \textbf{Proof:} Let $ \epsilon > 0 $. Choose $\delta = \epsilon$. Then, for $ 0 < \left| x - 3 \right| < \delta $, we have
    \begin{align*}
        \left| \frac{3x+1}{4x+3} - \frac{2}{3}\right| = \left| \frac{x-3}{12x+9} \right| < |x-3| < \delta = \epsilon
    \end{align*}
    However, we must justify our claim that $ \left| \frac{x-3}{12x+9} \right| < |x-3| $. For this to be the case, we have that $|12x + 9| > 1$. Notice that as the limit approaches 3, we have that $|12x + 9| = |12(3) + 9| = 45 > 1$. This works for all values of $x$ around 3, therefore justifying the claim above. \\
    Thus, $ \lim_{x \to 3} (\frac{3x+1}{4x+3}) = \frac{2}{3} $. \hfill $\Box$

\end{document}